src/code/kubernetes_model/simplereplicaset.v
@@ -117,17 +117,9 @@ Definition FilterPodsByOwnerⁱᵐᵖˡ : val :=
       do:  ("result" <-[#sliceT] "$r0")));;;
     return: (![#sliceT] "result", #interface.nil)).
 
-Definition IsPodActive : go_string := "kubernetes_model/simplereplicaset.IsPodActive"%go.
-
-(* go: replica_set.go:58:6 *)
-Definition IsPodActiveⁱᵐᵖˡ : val :=
-  λ: "p",
-    exception_do (let: "p" := (mem.alloc "p") in
-    return: (((v1.PodSucceeded ≠ (![#v1.PodPhase] (struct.field_ref #v1.PodStatus #"Phase"%go (struct.field_ref #v1.Pod #"Status"%go (![#ptrT] "p"))))) && (v1.PodFailed ≠ (![#v1.PodPhase] (struct.field_ref #v1.PodStatus #"Phase"%go (struct.field_ref #v1.Pod #"Status"%go (![#ptrT] "p")))))) && ((![#ptrT] (struct.field_ref #v1.ObjectMeta #"DeletionTimestamp"%go (struct.field_ref #v1.Pod #"ObjectMeta"%go (![#ptrT] "p")))) = #null))).
-
 Definition FilterActivePods : go_string := "kubernetes_model/simplereplicaset.FilterActivePods"%go.
 
-(* go: replica_set.go:64:6 *)
+(* go: replica_set.go:56:6 *)
 Definition FilterActivePodsⁱᵐᵖˡ : val :=
   λ: "pods",
     exception_do (let: "pods" := (mem.alloc "pods") in
@@ -138,7 +130,7 @@ Definition FilterActivePodsⁱᵐᵖˡ : val :=
       do:  ("p" <-[#ptrT] "$value");;;
       do:  "$key";;;
       (if: let: "$a0" := (![#ptrT] "p") in
-      (func_call #IsPodActive) "$a0"
+      (func_call #controller.IsPodActive) "$a0"
       then
         let: "$r0" := (let: "$a0" := (![#sliceT] "result") in
         let: "$a1" := ((let: "$sl0" := (![#ptrT] "p") in
@@ -150,7 +142,7 @@ Definition FilterActivePodsⁱᵐᵖˡ : val :=
 
 Definition manageReplicas : go_string := "kubernetes_model/simplereplicaset.manageReplicas"%go.
 
-(* go: replica_set.go:74:6 *)
+(* go: replica_set.go:66:6 *)
 Definition manageReplicasⁱᵐᵖˡ : val :=
   λ: "activePods" "rs",
     exception_do (let: "rs" := (mem.alloc "rs") in
@@ -218,7 +210,7 @@ Definition manageReplicasⁱᵐᵖˡ : val :=
 
 Definition syncReplicaSet : go_string := "kubernetes_model/simplereplicaset.syncReplicaSet"%go.
 
-(* go: replica_set.go:102:6 *)
+(* go: replica_set.go:94:6 *)
 Definition syncReplicaSetⁱᵐᵖˡ : val :=
   λ: "namespace" "name",
     exception_do (let: "name" := (mem.alloc "name") in
@@ -266,7 +258,7 @@ Definition syncReplicaSetⁱᵐᵖˡ : val :=
 
 Definition vars' : list (go_string * go_type) := [(state, ptrT)].
 
-Definition functions' : list (go_string * val) := [(CreatePod, CreatePodⁱᵐᵖˡ); (FilterPodsByOwner, FilterPodsByOwnerⁱᵐᵖˡ); (IsPodActive, IsPodActiveⁱᵐᵖˡ); (FilterActivePods, FilterActivePodsⁱᵐᵖˡ); (manageReplicas, manageReplicasⁱᵐᵖˡ); (syncReplicaSet, syncReplicaSetⁱᵐᵖˡ)].
+Definition functions' : list (go_string * val) := [(CreatePod, CreatePodⁱᵐᵖˡ); (FilterPodsByOwner, FilterPodsByOwnerⁱᵐᵖˡ); (FilterActivePods, FilterActivePodsⁱᵐᵖˡ); (manageReplicas, manageReplicasⁱᵐᵖˡ); (syncReplicaSet, syncReplicaSetⁱᵐᵖˡ)].
 
 Definition msets' : list (go_string * (list (go_string * val))) := [].
 
